Stuck on helping proof - merge with master when get_tid is added

helping/HelpingOn.v
@@ -1,14 +1,80 @@
 Require Import CRIS SchHeader.
+From iris.algebra Require Import gmap_view.
 From CRIS.helping Require Import Header.
+From stdpp Require Import fin_sets.
 
+(* Resource algebra for the helping module *)
+(* Class helpingG `{!crisG Γ Σ α β τ _S _I} (jobID : Type) := {
+  helping_tokG :: inG (gmap_viewR nat (agreeR (leibnizO jobID))) Γ
+}.
+Definition helpingΓ (jobID : Type) : HRA :=
+  #[gmap_viewR nat (agreeR (leibnizO jobID))].
+Global Instance subG_helpingΓ `{!crisG Γ Σ α β τ _S _I} (jobID : Type) :
+  subG (helpingΓ jobID) Γ → helpingG jobID.
+Proof. solve_inG. Defined.
+Hint Unfold subG_helpingΓ : GRA_index.
+
+Section resource.
+  Context `{!crisG Γ Σ α β τ _S _I, !helpingG jobID}.
+
+  Definition helping_tok (tid : nat) (jid : jobID) : iProp Σ :=
+    own base_γ (gmap_view_frag (V:=agreeR $ leibnizO jobID) tid (DfracOwn 1) (to_agree jid)).
+End resource. *)
+Section HoareCall.
+  Context {Σ : GRA}.
+
+  Definition fspec_option_meta (fspo : option fspec) : Type :=
+    match fspo with
+    | Some fsp => meta fsp
+    | None => unit
+    end.
+
+  Definition HoareCall_prologue fspo parg : itree crisE (fspec_option_meta fspo * Any.t) :=
+    Seal.sealing "Help"
+    (match fspo as fspo return itree crisE (fspec_option_meta fspo * Any.t) with
+    | Some fsp =>
+        x <- trigger (Choose (meta fsp));;
+        varg <- trigger (Choose Any.t);;
+        trigger (Guarantee (precond fsp x parg varg));;;
+        Ret (x, varg)
+    | None => Ret (tt, parg)
+    end).
+
+  Definition HoareCall_epilogue fspo (x : fspec_option_meta fspo) (pret : Any.t)
+      : itree crisE Any.t :=
+    Seal.sealing "Help"
+    (match fspo as fspo return fspec_option_meta fspo → itree crisE Any.t with
+    | Some fsp =>
+        λ x,
+          vret <- trigger (Take Any.t);;
+          trigger (Assume (postcond fsp x vret pret));;;
+          Ret vret
+    | None => λ _, Ret pret
+    end) x.
+
+  Lemma HoareCall_unfold fspo :
+    SModTr.HoareCall SchHdr.yield (()↑) fspo =
+    xarg <- HoareCall_prologue fspo (()↑);;
+    ret <- trigger (Call SchHdr.yield xarg.2);;
+    HoareCall_epilogue fspo xarg.1 ret.
+  Proof.
+    rewrite /SModTr.HoareCall /HoareCall_prologue /HoareCall_epilogue; unseal "Help".
+    destruct fspo as [fsp|]; ss.
+    { ired. f_equal. extensionalities x. ired. f_equal. extensionalities arg. ired. f_equal.
+      extensionalities t. f_equal. extensionalities a. unseal "Help". done. }
+    { ired. erewrite <-bind_ret_r at 1. f_equal. extensionalities a. unseal "Help". done. }
+  Qed.
+End HoareCall.
+
+(* Helping module *)
 Module HelpingOn. Section HelpingOn.
-
-  Context `{Σ : GRA}.
+  Context {Σ : GRA} {jobID : Type}.
 
   Context (mn : string).
-  Context {jobID : Type} (jobcode : jobID → itree Helping.pureE unit).
+  Context (jobcode : jobID → itree Helping.pureE unit).
 
-  Definition jobmap : Type := gmap nat jobID.
+  Variant progress := Pend | InProgress.
+  Definition jobmap : Type := gmap nat (jobID * progress).
 
   Definition scopes := [mn].
   Definition v_reqs := mn ↯ "reqs".
@@ -16,42 +82,50 @@ Module HelpingOn. Section HelpingOn.
   Definition try_run (tid : nat) : itree crisE Any.t :=
     'reqs : jobmap <- cgetU v_reqs;;
     match reqs !! tid with
-    | None => Ret ()↑
-    | Some jid =>
-        cput v_reqs (delete tid reqs);;;
+    | Some (jid, Pend) =>
+        cput v_reqs (<[tid := (jid, InProgress)]> reqs);;;
         Helping.trans (jobcode jid);;;
+        cput v_reqs (delete tid reqs);;;
         Ret ()↑
+    | _ => Ret ()↑
     end.
 
-  Definition run: Any.t → itree crisE Any.t :=
+  Definition run : Any.t → itree crisE Any.t :=
     λ arg,
       'jid : jobID <- arg↓?;;
-      'tid : nat <- ccallU SchHdr.get_tid ();;
       'reqs : jobmap <- cgetU v_reqs;;
-      cput v_reqs (<[tid := jid]> reqs);;;
-      𝒴;;;
+      let tid := fresh (dom reqs) in
+      cput v_reqs (<[tid := (jid, Pend)]> reqs);;;
+      iterC (λ _ : (),
+        𝒴;;;
+        'reqs : jobmap <- cgetU v_reqs;;
+        match reqs !! tid with
+        | Some (jid, InProgress) => Ret (inl tt)
+        | _ => Ret (inr tt↑)
+        end
+      ) ();;;
       try_run tid.
 
-  Definition help: Any.t → itree crisE Any.t :=
+  Definition help (sp : sp_type) : Any.t → itree crisE Any.t :=
     λ _,
-      𝒴;;;
       tid <- trigger (Choose nat);;
+      xarg <- HoareCall_prologue (sp SchHdr.yield) (() ↑);;
+      HoareCall_epilogue (sp SchHdr.yield) xarg.1 (() ↑);;;
       try_run tid;;;
       𝒴;;;
       Ret ()↑.
 
-  Definition fnsems : alist (option string) (fnsem_type (option fspec * fbody)) :=
-    [(Some (Helping.run mn),  (false, wmask_all, scopes, (None, run)));
-     (Some (Helping.help mn), (false, wmask_all, scopes, (None, help)))].
+  Definition fnsems (sp : sp_type) : alist (option string) (fnsem_type (option fspec * fbody)) :=
+    [(Some (Helping.run mn),  (true, wmask_all, scopes, (None, run)));
+     (Some (Helping.help mn), (true, wmask_all, scopes, (None, help sp)))].
 
-  Program Definition Mod: SMod.t := {|
+  Program Definition Mod (sp : sp_type) : SMod.t := {|
     SMod.scopes := scopes;
-    SMod.fnsems := fnsems;
+    SMod.fnsems := fnsems sp;
     SMod.initial_st := [(v_reqs, (∅ : jobmap)↑)];
   |}.
   Solve All Obligations with prove_scope.
   Next Obligation. prove_nodup. Qed.
 
-  Definition t sp : Mod.t := Seal.sealing CRIS (SMod.to_mod sp Mod).
-
+  Definition t sp : Mod.t := Seal.sealing CRIS (SMod.to_mod sp (Mod sp)).
 End HelpingOn. End HelpingOn.
