helping/HelpingOnOffproof.v
@@ -1,19 +1,12 @@
 Require Import CRIS.
 Require Import LMod.
 Require Import GSim GSimFacts GSimTactics.
-Require Import SchHeader SchA.
+Require Import SchHeader SchI.
 From CRIS.helping Require Import Header HelpingOn HelpingOff.
 
-Section Helping.
-  Context `{!crisG Γ Σ α β τ _S _I, !schG}.
-  Context (sp : sp_type) (mn : string). (* sp, module name for the helping module *)
-  Context {jobID : Type} (jobs : jobID → itree Helping.pureE unit).
-  Context (sp_s : sp_type) (sp_u : spl_type).
-  Context (msk : string → bool). (* mask for the user module *)
+Section auxilliary.
 
-  Local Definition mod_on :=  (HelpingOn.t mn jobs sp)  ★ (CFilter.filter msk (SchA.t sp_s sp_u)).
-  Local Definition mod_off := (HelpingOff.t mn jobs sp) ★ (CFilter.filter msk (SchA.t sp_s sp_u)).
-
+  Context {Σ : GRA}.
 
   Lemma Red_vis_Assume {R} P (ktr : () → itree crisE R) :
     ModTr.trans (vis (Events.Assume P) ktr) =
@@ -32,6 +25,8 @@ Section Helping.
     eapply observe_eta; ss. f_equal. extensionality x. ss.
   Qed.
 
+End auxilliary.
+
   Tactic Notation "red_bind" tactic(tac) :=
     lazymatch goal with
     | [ |- @ITree.bind _ _ _ ?itr _ = _ ] =>
@@ -43,7 +38,7 @@ Section Helping.
         | guaranteeK _ _ => eapply guaranteeK_bind
         | unwrapUK _ _ => eapply unwrapUK_bind
         | unwrapNK _ _ => eapply unwrapNK_bind
-        | UpdateProphK _ _ _ _ => eapply UpdateProphK_bind
+        | RealUpdateK _ _ => eapply RealUpdateK_bind
         | SBRed.putSB _ _ _ _ _ _ => eapply SBRed.putSB_bind
         | SBRed.getSB _ _ _ _ _ => eapply SBRed.getSB_bind
         | SBRed.callSB _ _ _ _ _ _ => eapply SBRed.callSB_bind
@@ -91,8 +86,8 @@ Section Helping.
             eapply SBRed.unwrapUK
         | unwrapNK _ _ =>
             eapply SBRed.unwrapNK
-        | UpdateProphK _ _ _ _ =>
-            eapply SBRed.update_prophK
+        | RealUpdateK _ _ _ =>
+            eapply SBRed.ruK
         | @ITree.bind _ _ _ _ _ =>
             eapply SBRed.bind
         | _ =>
@@ -151,8 +146,8 @@ Section Helping.
             eapply SRed.unwrapUK
         | unwrapNK _ _ =>
             eapply SRed.unwrapNK
-        | UpdateProphK _ _ _ _ =>
-            eapply SRed.update_prophK
+        | RealUpdateK _ _ _ =>
+            eapply SRed.ruK
         | @ITree.bind _ _ _ _ _ =>
             eapply SRed.bind
         | _ =>
@@ -235,7 +230,7 @@ Tactic Notation "red_ModTr" tactic(tac) :=
           eapply SRed.guaranteeK
       | unwrapNK _ _ =>
           eapply SRed.unwrapNK
-      | UpdateProphK _ _ _ _ =>
+      | RealUpdateK _ _ _ _ =>
           eapply SRed.update_prophK
       | @ITree.bind _ _ _ _ _ =>
           eapply SRed.bind *)
@@ -336,8 +331,8 @@ Tactic Notation "red_ModTr" tactic(tac) :=
         eapply unwrapU_unwrapUK
     | [ |- unwrapN _ = _ ] =>
         eapply unwrapN_unwrapNK
-    | [ |- UpdateProph _ _ _ = _ ] =>
-        eapply UpdateProph_UpdateProphK
+    | [ |- RealUpdate _ _ = _ ] =>
+        eapply RealUpdate_RealUpdateK
     | [ |- SModTr.HoareCall _ _ _ = _ ] =>
         unfold SModTr.HoareCall;
         _gnorm_itr
@@ -408,16 +403,195 @@ Tactic Notation "red_ModTr" tactic(tac) :=
   Ltac step_l :=
     norm_l; guclo gsim_indC_spec; econs; instantiate (1:=smj_top).
 
-  Theorem helping_onoff_correct E q
-      (SchInSp : sp_incl (SchAS.sp sp_u E q) sp_s) :
+  Ltac replace_tp_r :=
+    match goal with
+    | |- gpaco7 _ _ _ _ _ _ _ _ _ _ (LModTr.interp_stateE _ (iterV _ ?tp) _) =>
+        pattern tp;
+        match goal with
+        | |- ?f ?tp =>
+            eapply (eq_ind_r f); cycle 1
+        end
+    end.
+  Ltac replace_tp_l :=
+    match goal with
+    | |- gpaco7 _ _ _ _ _ _ _ _ _ (LModTr.interp_stateE _ (iterV _ ?tp) _) _ =>
+        pattern tp;
+        match goal with
+        | |- ?f ?tp =>
+            eapply (eq_ind_r f); cycle 1
+        end
+    end.
+
+Section Helping.
+  Context `{!crisG Γ Σ α β τ _S _I, !schG}.
+  Context (sp : sp_type) (mn : string). (* sp, module name for the helping module *)
+  Context {jobID : Type} (jobs : jobID → itree Helping.pureE unit).
+  (* Context (sp_s : sp_type) (sp_u : spl_type). *)
+  Context (msk : string → bool). (* mask for the user module *)
+
+  Local Definition mod_on :=  (HelpingOn.t mn jobs sp)  ★ (CFilter.filter msk (SchI.t)).
+  Local Definition mod_off := (HelpingOff.t mn jobs sp) ★ (CFilter.filter msk (SchI.t)).
+
+  Local Lemma get_tid_run_neq : SchHdr.get_tid ≠ Helping.run mn.
+  Proof.
+    rewrite /SchHdr.get_tid /Helping.run; destruct (decide (String.length mn = 7)) as [Hlen|];
+      cycle 1.
+    { assert (Hlen : String.length "Sch.get_tid" = 11) by ss.
+      intros Heq; rewrite Heq string_length_app in Hlen; ss; lia.
+    }
+    rewrite -get_correct; intros Hfalse; specialize (Hfalse (3 + String.length mn)).
+    rewrite -(append_correct2 _ _) Hlen in Hfalse; ss.
+  Qed.
+
+  Local Lemma get_tid_help_neq : SchHdr.get_tid ≠ Helping.help mn.
+  Proof.
+    rewrite /SchHdr.get_tid /Helping.help; destruct (decide (String.length mn = 6)) as [Hlen|];
+      cycle 1.
+    { assert (Hlen : String.length "Sch.get_tid" = 11) by ss.
+      intros Heq; rewrite Heq string_length_app in Hlen; ss; lia.
+    }
+    rewrite -get_correct; intros Hfalse; specialize (Hfalse (3 + String.length mn)).
+    rewrite -(append_correct2 _ _) Hlen in Hfalse; ss.
+  Qed.
+
+  Local Lemma yield_run_neq : SchHdr.yield ≠ Helping.run mn.
+  Proof.
+    rewrite /SchHdr.yield /Helping.run; destruct (decide (String.length mn = 5)) as [Hlen|];
+      cycle 1.
+    { assert (Hlen : String.length "Sch.yield" = 9) by ss.
+      intros Heq; rewrite Heq string_length_app in Hlen; ss; lia.
+    }
+    rewrite -get_correct; intros Hfalse; specialize (Hfalse (3 + String.length mn)).
+    rewrite -(append_correct2 _ _) Hlen in Hfalse; ss.
+  Qed.
+
+  Local Lemma yield_help_neq : SchHdr.yield ≠ Helping.help mn.
+  Proof.
+    rewrite /SchHdr.yield /Helping.help; destruct (decide (String.length mn = 4)) as [Hlen|];
+      cycle 1.
+    { assert (Hlen : String.length "Sch.yield" = 9) by ss.
+      intros Heq; rewrite Heq string_length_app in Hlen; ss; lia.
+    }
+    rewrite -get_correct; intros Hfalse; specialize (Hfalse (0 + String.length mn)).
+    rewrite -(append_correct2 _ _) Hlen in Hfalse; ss.
+  Qed.
+
+  Lemma yield_unfold :
+    @Sch.yield crisE _ _ =
+    tau;; b <- trigger (Choose (option bool));;
+    match b with
+    | None => Ret tt
+    | Some false => Sch.yield
+    | Some true => trigger (Call SchHdr.yield tt↑);;; Sch.yield
+    end.
+  Proof.
+    rewrite {1}/Sch.yield; unseal "Sch"; rewrite unfold_iterC.
+    repeat f_equal. ired. repeat f_equal. extensionalities b. destruct b as [[|]|]; ss.
+    { ired. f_equal. extensionalities x. rewrite /Sch.yield; unseal "Sch"; ss. }
+    { ired. rewrite /Sch.yield; unseal "Sch"; ss. }
+    { ired. done. }
+  Qed.
+
+  Definition to_reqlist
+      (tl : list (itree lmodE Any.t * itree lmodE Any.t * option (nat * jobID * option bool)))
+      : list (nat * (jobID * HelpingOn.progress)) :=
+    (omap (λ n,
+                match n with
+                | Some (tid, jid, None) => Some (tid, (jid, HelpingOn.Pend))
+                | Some (tid, jid, Some _) => Some (tid, (jid, HelpingOn.InProgress))
+                | None => None
+                end) tl.*2).
+
+  Definition to_reqmap tl : gmap nat (jobID * HelpingOn.progress) := list_to_map (to_reqlist tl).
+
+  Notation "'⇓cris'" := (interpV (ModTr.handle_crisE)).
+  Notation "'⇓sb(' i ',' m ',' s ')'" := (interpV (SB.handle_sandbox i m s)).
+  Notation "'⇓smod(' sp ')'" := (interpV (SModTr.handle sp)).
+
+  Definition yield_epliogue (tid_cur : nat) : itree lmodE Any.t :=
+    ⇓cris (⇓sb(false, wmask_and msk wmask_all, SchI.scopes) (⇓smod(sp_none) (
+        x <- cput SchI.SchI.v_tid tid_cur;;
+        Ret (x↑)
+    ))).
+  (* Definition yield_epliogue (tid_cur : nat) (x : meta (SchAS.yield_spec ⊤ 1)): itree lmodE Any.t :=
+    ⇓cris (⇓sb(true, wmask_and msk wmask_all, SchA.scopes) (
+      r <- ⇓smod(sp_s) (
+        cput SchI.SchI.v_tid tid_cur;;;
+        r <- SchA.check_internal;;
+        Ret (r↑)
+      );;
+      ret <- trigger (Choose Any.t);;
+      trigger (Guarantee (postcond (SchAS.yield_spec ⊤ 1) x r ret));;;
+      Ret ret
+    )). *)
+
+  Definition helpee_pend_s
+      (tid_cur : nat) (j : jobID) img_c msk_c scp_c k
+      (fspo : option fspec) (x_fsp : fspec_option_meta fspo)
+      : itree lmodE Any.t :=
+    x <- yield_epliogue tid_cur;; tau;;
+    r <- ⇓cris (⇓sb(true, wmask_all, HelpingOff.scopes mn) (
+      HoareCall_epilogue fspo x_fsp x;;;
+      ⇓smod(sp) (𝒴;;; Helping.trans (jobs j);;; Ret ()↑)
+    ));; tau;;
+    ⇓cris (⇓sb(img_c, msk_c, scp_c) (k r)).
+
+  Definition loop_t (stid_cur : nat) : () → itree crisE (() + Any.t) :=
+    λ _ : (),
+      'x_ : HelpingOn.jobmap <- cgetU (HelpingOn.v_reqs mn);;
+      match x_ !! stid_cur with
+      | Some y =>
+          let (_, y0) := (y : jobID * HelpingOn.progress) in
+          match y0 with
+          | HelpingOn.Pend => Ret (inr () ↑)
+          | HelpingOn.InProgress => Ret (inl ())
+          end
+      | None => Ret (inr () ↑)
+      end.
+
+  Definition helpee_pend_t
+      (tid_cur tid_stid_cur : nat) (j : jobID) img_c msk_c scp_c k
+      (fspo : option fspec) (x_fsp : fspec_option_meta fspo)
+      : itree lmodE Any.t :=
+    x <- yield_epliogue tid_cur;; tau;;
+    r <- ⇓cris (⇓sb(true, wmask_all, HelpingOff.scopes mn) (
+      HoareCall_epilogue fspo x_fsp x;;;
+      ⇓smod(sp) (
+        𝒴;;; x <- loop_t tid_stid_cur ();;
+        match x with
+        | inl l => tau;; ITree.iter (λ _ : (), x <- 𝒴;; loop_t tid_stid_cur x) l
+        | inr r => Ret r
+        end;;;
+        HelpingOn.try_run mn jobs tid_stid_cur)
+    ));; tau;;
+    ⇓cris (⇓sb(img_c, msk_c, scp_c) (k r)).
+
+  Definition help_rel
+      (itr_s itr_t : itree lmodE Any.t) (no : option (nat * jobID * option bool)) : Prop :=
+    match no with
+    | None =>
+        ∃ itr img msk scp,
+          itr_s = itr_t ∧ itr_s = ModTr.trans (SB.sandbox img msk scp itr)
+    | Some (tid, jid, None) =>
+        ∃ tid_cur img_c msk_c scp_c k fsp x_fsp,
+          itr_s = helpee_pend_s tid_cur jid img_c msk_c scp_c k fsp x_fsp ∧
+          itr_t = helpee_pend_t tid_cur tid jid img_c msk_c scp_c k fsp x_fsp (* pending *)
+    | Some (tid, jid, Some b) =>
+        if b : bool
+        then itr_s = Ret tt↑ ∧ itr_t = Ret tt↑ (* helpee *)
+        else itr_s = Ret tt↑ ∧ itr_t = Ret tt↑ (* helper *)
+    end.
+
+  Theorem helping_onoff_correct :
+      (* (SchInSp : sp_incl (SchAS.sp sp_u E q) sp_s) : *)
     ctx_refines (mod_off, emp%I) (mod_on, emp%I).
   Proof.
     rewrite /mod_off /mod_on.
     intros [ctx ctxP] WF; ss; split.
     { inv WF.
       econs.
-      { revert wf_fns. rewrite /HelpingOff.t /HelpingOn.t /SchA.t; unseal CRIS; ss. }
-      { revert wf_scopes. rewrite /HelpingOff.t /HelpingOn.t /SchA.t; unseal CRIS; ss. }
+      { revert wf_fns. rewrite /HelpingOff.t /HelpingOn.t /SchI.t; unseal CRIS; ss. }
+      { revert wf_scopes. rewrite /HelpingOff.t /HelpingOn.t /SchI.t; unseal CRIS; ss. }
     }
     intros rs Hval Hrs; exists rs; split; [exact Hval|split; [done|]].
 
@@ -428,42 +602,748 @@ Tactic Notation "red_ModTr" tactic(tac) :=
     destruct (alist_find None fnsems) eqn: FIND; s; cycle 1.
     { s. ired. ginit. gstep. econs. econs. ss. }
     rewrite alist_find_app_o; des_ifs.
-    { rewrite alist_find_app_o /HelpingOn.t /SchA.t in Heq; revert Heq; unseal CRIS; intros Heq.
+    { rewrite alist_find_app_o /HelpingOn.t /SchI.t in Heq; revert Heq; unseal CRIS; intros Heq.
       des_ifs; ss.
     }
     subst fnsems; rewrite alist_find_app_o in FIND; des_ifs.
-    { rewrite /HelpingOff.t /SchA.t in Heq0; revert Heq0; unseal CRIS; ss. }
+    { rewrite /HelpingOff.t /SchI.t in Heq0; revert Heq0; unseal CRIS; ss. }
     rewrite FIND /ModTr.trans_ktree; ired.
 
     destruct f as [[[imgf mskf] scpf] f].
 
-    clear Heq Heq0 FIND.
+    clear Heq Heq0.
     rewrite /SB.sandbox_body /=.
 
     ginit. guclo bindC_spec. econs; cycle 1.
     { instantiate (1:=λ r_s r_t, r_s.2 = r_t.2). ii; gstep; ss. subst; econs; econs; ss. }
 
-    move imgf at top. move mskf at top. move scpf at top.
-    generalize (f arg) as f'; clear arg f; intros f.
+    rewrite /HelpingOff.t /HelpingOn.t /SchI.t; unseal CRIS; ss.
+    set (st_src := (_, _) :: _) at 1.
+    set (st_tgt := (_, _) :: _).
+    set (tp_src := (0, [_])) at 1.
+    set (tp_tgt := (0, [_])).
     clear Hrs.
+    cut
+      (∃ (tl : list (itree lmodE Any.t * itree lmodE Any.t * option (nat * jobID * option bool)))
+      (tid_cur stid_cur : nat) (ths : list (nat * option SAny.t)) (b_sch : bool) st_ctx,
+        st_src = [(SchI.SchI.v_ths, ths↑);
+          (SchI.SchI.v_tid, tid_cur↑); (SchI.SchI.v_tids, (map fst ths)↑)] ++ st_ctx ∧
+        st_tgt = [(HelpingOn.v_reqs mn, (to_reqmap tl)↑); (SchI.SchI.v_ths, ths↑);
+          (SchI.SchI.v_tid, tid_cur↑); (SchI.SchI.v_tids, (map fst ths)↑)] ++ st_ctx ∧
+        tp_src = (stid_cur, (fst ∘ fst) <$> tl) ∧ tp_tgt = (stid_cur, (snd ∘ fst) <$> tl) ∧
+        List.NoDup (to_reqlist tl).*1 ∧
+        ∀ i itr_s itr_t no, tl !! i = Some (itr_s, itr_t, no) → help_rel itr_s itr_t no); cycle 1.
+    { esplits; subst st_src st_tgt; ss; repeat f_equal; first instantiate (1:=[(_,_, None)]); ss.
+      { econs; ss; econs. }
+      intros ???? [-> In]%list_lookup_singleton_Some; clarify.
+      r. esplits; eauto.
+    }
+    generalize st_src, st_tgt, tp_src, tp_tgt.
+    clear st_src st_tgt tp_src tp_tgt f imgf mskf scpf FIND arg.
+    (* generalize f. *)
     revert_until WF.
     gcofix CIH.
-    intros rs Hrs f.
+    intros rs Hrs ???? [tl [tid_cur [stid_cur [ths [b_sch [st_ctx [-> [-> [-> [-> [Htl Hlookup]]]]]]]]]]].
 
-    destruct (case_itrH f) as [[v ->]|Hf].
-    { 
-      ziter_l; zstep_l.
-      ziter_r; zstep_r.
-      zstep; rewrite /HelpingOff.t /HelpingOn.t /SchA.t; unseal CRIS; ss.
+    iter_l; destruct (_ !! _) as [i|] eqn : Htid; cycle 1.
+    { step_l. norm_l. step_l. ss. }
+
+    apply list_lookup_fmap_inv in Htid as [[[itr_src itr_tgt] no] [-> Htid]]; s.
+    iter_r. rewrite list_lookup_fmap Htid /=.
+    destruct no as [|]; cycle 1.
+    { apply lookup_lt_Some in Htid as Htid_cur.
+      pose proof Htid as Htid'. apply Hlookup in Htid' as [itr_c [img_c [msk_c [scp_c [-> ->]]]]].
+      destruct (case_itrH itr_c) as [[v ->]|Hf]; ss.
+      {
+        norm_l. step_l. norm_r. step_r.
+        des_ifs; ss; cycle 1.
+        { norm_l. step_l. ss. }
+        norm_l. norm_r.
+        zstep; rewrite /HelpingOff.t /HelpingOn.t /SchI.t; unseal CRIS; ss.
+      }
+      destruct Hf as [[f' ->]|Hf].
+      { zprogress. norm_l. norm_r. step_l; step_r.
+        norm_l. norm_r.
+        gbase. eapply CIH; eauto.
+        eexists (<[stid_cur := (_, _, None)]> tl); esplits; eauto.
+        { erewrite <-(take_drop_middle tl stid_cur) at 1; eauto.
+          rewrite insert_take_drop; last ss.
+          rewrite /to_reqmap /to_reqlist /= ?fmap_app ?omap_app /=. refl.
+        }
+        { rewrite list_fmap_insert //=. }
+        { rewrite list_fmap_insert //=. }
+        { rewrite insert_take_drop //= /to_reqlist fmap_app fmap_cons omap_app /=.
+          move: Htl; erewrite <-(take_drop_middle tl stid_cur) at 1; eauto.
+          rewrite /to_reqlist fmap_app omap_app //=.
+        }
+        { intros i; destruct (decide (i = stid_cur)); subst; cycle 1.
+          { intros ???; rewrite list_lookup_insert_ne //=; apply Hlookup. }
+          { rewrite list_lookup_insert; ii; clarify; r; esplits; eauto. }
+        }
+      }
+      destruct Hf as [[P [f' ->]]|Hf].
+      { destruct img_c; cycle 1.
+        { norm_l. step_l. ss. }
+        zprogress.
+        norm_l; norm_r.
+        step_l. step_r. norm_l; norm_r. hss.
+        iter_l. rewrite list_lookup_insert /=. hss. norm_l. step_l.
+        intros res; norm_l. step_l. norm_l.
+        rewrite list_insert_insert. 2:{ rewrite length_fmap //. }
+        iter_l. rewrite list_lookup_insert /=; [|rewrite length_fmap //].
+        step_l. intros Hres. norm_l. step_l. norm_l.
+        rewrite list_insert_insert.
+        iter_l. rewrite list_lookup_insert /=; [|rewrite length_fmap //]. step_l. norm_l.
+        rewrite list_insert_insert.
+        iter_l. rewrite list_lookup_insert /=; [|rewrite length_fmap //]. hss.
+        norm_l. step_l. norm_l. ired.
+        rewrite list_insert_insert.
+
+        iter_r. rewrite list_lookup_insert /=; [|rewrite length_fmap //]. hss. norm_r. step_r.
+        exists res; norm_r. step_r. norm_r.
+        rewrite list_insert_insert.
+        iter_r. rewrite list_lookup_insert /=; [|rewrite length_fmap //].
+        step_r. unshelve eexists; eauto. norm_r. step_r. norm_r.
+        rewrite list_insert_insert.
+        iter_r. rewrite list_lookup_insert /=; [|rewrite length_fmap //]. step_r. norm_r.
+        rewrite list_insert_insert.
+        iter_r. rewrite list_lookup_insert /=; [|rewrite length_fmap //]. hss.
+        norm_r. step_r. norm_r. ired.
+        rewrite list_insert_insert.
+        gbase. eapply (CIH res); eauto.
+        eexists (<[stid_cur := (_, _, None)]> tl); esplits; eauto.
+        { erewrite <-(take_drop_middle tl stid_cur) at 1; eauto.
+          rewrite insert_take_drop; last ss.
+          rewrite /to_reqmap /to_reqlist /= ?fmap_app ?omap_app /=. refl.
+        }
+        { rewrite list_fmap_insert //=. }
+        { rewrite list_fmap_insert //=. }
+        { rewrite insert_take_drop //= /to_reqlist fmap_app fmap_cons omap_app /=.
+          move: Htl; erewrite <-(take_drop_middle tl stid_cur) at 1; eauto.
+          rewrite /to_reqlist fmap_app omap_app //=.
+        }
+        { intros i; destruct (decide (i = stid_cur)); subst; cycle 1.
+          { intros ???; rewrite list_lookup_insert_ne //=; apply Hlookup. }
+          { rewrite list_lookup_insert; ii; clarify; r; esplits; eauto. }
+        }
+      }
+      destruct Hf as [[res [f' ->]]|Hf].
+      { admit. (* AssumeRes *) }
+      destruct Hf as [[P [f' ->]]|Hf].
+      { admit. (* Guarantee *) }
+      destruct Hf as [[R [[fn args|fn args|tid_yield] [k ->]]]|Hf].
+      {
+        ss; destruct (msk_c fn); cycle 1.
+        { norm_l. step_l. ss. }
+        ss. zprogress.
+
+        step_l. step_r.
+        destruct (decide (fn = Helping.run mn)); subst.
+        { (* Helping.run *)
+          norm_l. norm_r.
+          rewrite {1 3}/LMod.prog ?alist_find_map_snd /=.
+          destruct (dec _ _) as [?|e]; [ss|clarify].
+          norm_l. norm_r.
+
+          iter_r. rewrite list_lookup_insert /=; [|rewrite length_fmap //]. step_r. norm_r.
+          rewrite list_insert_insert.
+          rewrite /HelpingOn.run /HelpingOff.run.
+          destruct (args↓) as [j|] eqn:Hargs ; cycle 1.
+          { iter_l. rewrite list_lookup_insert /=; [|rewrite length_fmap //].
+            step_l. norm_l. rewrite list_insert_insert.
+            rewrite Hargs /=.
+            iter_l. rewrite list_lookup_insert /=; [|rewrite length_fmap //].
+            norm_l; step_l; ss.
+          }
+          ss.
+          rewrite /ModTr.trans_ktree /SB.sandbox_body /= Hargs.
+
+          iter_l. rewrite list_lookup_insert /=; [|rewrite length_fmap //].
+          rewrite list_insert_insert.
+          step_l. norm_l. ired.
+
+          (* call for help *)
+          iter_r. rewrite list_lookup_insert /=; [|rewrite length_fmap //].
+          rewrite String.eqb_refl /=. step_r. norm_r. hss. rewrite ModTr.alist_encode_decode.
+          rewrite list_insert_insert.
+          ss. destruct (dec _ _) as [e|]; ss; clear e.
+          iter_r. rewrite list_lookup_insert /=; [|rewrite length_fmap //].
+          hss. rewrite String.eqb_refl /=. norm_r. step_r. norm_r. hss.
+          rewrite ModTr.alist_encode_decode /alist_upd /_alist_upd /=.
+          destruct (dec _ _) as [e|]; ss; clear e.
+          rewrite list_insert_insert.
+          iter_r. rewrite list_lookup_insert /=; [|rewrite length_fmap //]. step_r. norm_r.
+          rewrite list_insert_insert.
+          iter_r. rewrite list_lookup_insert /=; [|rewrite length_fmap //]. step_r. norm_r.
+          rewrite list_insert_insert.
+          ired.
+
+          fold (loop_t (fresh (dom (to_reqmap tl))) ()).
+          set (loop := λ _ : (), _) at 4.
+          assert (Heq : loop = loop_t (fresh (dom (to_reqmap tl)))); ss.
+          rewrite Heq; clear Heq loop.
+          rewrite (bisim_is_eq (unfold_iter _ _)).
+          ired.
+
+          gcofix CIH2.
+
+          rewrite {2}yield_unfold.
+          iter_r. rewrite list_lookup_insert /=; [|rewrite length_fmap //]. step_r. norm_r.
+          rewrite list_insert_insert.
+          iter_r. rewrite list_lookup_insert /=; [|rewrite length_fmap //].
+          norm_r. step_r.
+          intros [b|]; cycle 1.
+          { (* Loop exit *)
+            clear CIH2.
+            norm_r. step_r. norm_r.
+            rewrite list_insert_insert.
+            iter_r. rewrite list_lookup_insert /=; [|rewrite length_fmap //].
+            rewrite String.eqb_refl /=. step_r. norm_r. hss.
+            rewrite ?ModTr.alist_encode_decode.
+            rewrite list_insert_insert.
+            rewrite /alist_find eq_rel_dec_correct; des_ifs; ss.
+            ired. hss. ired. rewrite lookup_insert. ired.
+            iter_r. rewrite list_lookup_insert /=; [|rewrite length_fmap //].
+            rewrite String.eqb_refl /=. step_r. norm_r.
+            rewrite list_insert_insert.
+            hss. rewrite ModTr.alist_encode_decode /=.
+            destruct (dec _ _); ss.
+            ired. hss. ired. rewrite lookup_insert delete_insert.
+            2:{ rewrite -not_elem_of_dom; eapply is_fresh. }
+
+            iter_r. rewrite list_lookup_insert /=; [|rewrite length_fmap //].
+            rewrite String.eqb_refl /=. step_r. norm_r. hss.
+            rewrite list_insert_insert.
+            
+            iter_r. rewrite list_lookup_insert /=; [|rewrite length_fmap //].
+            step_r. norm_r. ired. rewrite ModTr.alist_encode_decode.
+            rewrite list_insert_insert.
+            rewrite /alist_upd /_alist_upd eq_rel_dec_correct; des_ifs.
+
+            rewrite yield_unfold.
+            iter_l. rewrite list_lookup_insert /=; [|rewrite length_fmap //].
+            step_l. norm_l.
+            rewrite list_insert_insert.
+
+            iter_l. rewrite list_lookup_insert /=; [|rewrite length_fmap //].
+            step_l. exists None. step_l. norm_l.
+            rewrite list_insert_insert.
+            ired.
+            gbase.
+            admit.
+            (* same tid doing same jobs *)
+          }
+          destruct b; cycle 1.
+          { zprogress. norm_r. step_r. norm_r. ired. rewrite list_insert_insert.
+            rewrite {1}yield_unfold.
+
+            iter_l. rewrite list_lookup_insert /=; [|rewrite length_fmap //].
+            step_l. norm_l. rewrite list_insert_insert.
+
+            iter_l. rewrite list_lookup_insert /=; [|rewrite length_fmap //].
+            step_l. exists (Some false). step_l. norm_l. ired.
+            rewrite list_insert_insert.
+            gbase.
+            eapply CIH2.
+          }
+
+          clear CIH2.
+          step_r. norm_r. rewrite list_insert_insert.
+
+          iter_r. rewrite list_lookup_insert /=; [|rewrite length_fmap //].
+          step_r. norm_r.
+          rewrite list_insert_insert.
+
+          rewrite {1}yield_unfold.
+
+          iter_l. rewrite list_lookup_insert /=; [|rewrite length_fmap //].
+          step_l. norm_l. rewrite list_insert_insert.
+
+          iter_l. rewrite list_lookup_insert /=; [|rewrite length_fmap //].
+          step_l. exists (Some true). norm_l. step_l. norm_l. rewrite list_insert_insert.
+
+          iter_l. rewrite list_lookup_insert /=; [|rewrite length_fmap //].
+          step_l. norm_l. rewrite list_insert_insert.
+
+          rewrite HoareCall_unfold. ired.
+          rewrite /HoareCall_prologue; unseal "Help".
+
+          destruct (sp SchHdr.yield) as [yield_spec|].
+          {
+            iter_r. rewrite list_lookup_insert /=; [|rewrite length_fmap //].
+            step_r. intros x. norm_r. step_r. norm_r.
+            rewrite list_insert_insert.
+
+            iter_r. rewrite list_lookup_insert /=; [|rewrite length_fmap //].
+            step_r. intros arg. norm_r. step_r. norm_r.
+            rewrite list_insert_insert.
+
+            iter_r. rewrite list_lookup_insert /=; [|rewrite length_fmap //].
+            step_r. norm_r.
+            rewrite list_insert_insert. hss. ired. hss. ired.
+
+            iter_r. rewrite list_lookup_insert /=; [|rewrite length_fmap //].
+            step_r. intros rs_2. norm_r. step_r. norm_r.
+            rewrite list_insert_insert.
+
+            iter_r. rewrite list_lookup_insert /=; [|rewrite length_fmap //].
+            step_r. intros Hrs_2. norm_r. step_r. norm_r.
+            rewrite list_insert_insert.
+
+            iter_r. rewrite list_lookup_insert /=; [|rewrite length_fmap //].
+            step_r. norm_r.
+            rewrite list_insert_insert. hss. ired. hss. ired.
+
+            iter_r. rewrite list_lookup_insert /=; [|rewrite length_fmap //].
+            step_r. norm_r.
+            rewrite list_insert_insert. ired.
+
+            iter_l. rewrite list_lookup_insert /=; [|rewrite length_fmap //].
+            step_l. exists x. norm_l. step_l. norm_l.
+            rewrite list_insert_insert.
+
+            iter_l. rewrite list_lookup_insert /=; [|rewrite length_fmap //].
+            step_l. exists arg. norm_l. step_l. norm_l.
+            rewrite list_insert_insert.
+
+            iter_l. rewrite list_lookup_insert /=; [|rewrite length_fmap //].
+            step_l. norm_l.
+            rewrite list_insert_insert. hss. ired. hss. ired.
+
+            iter_l. rewrite list_lookup_insert /=; [|rewrite length_fmap //].
+            step_l. exists rs_2. norm_l. step_l. norm_l.
+            rewrite list_insert_insert.
+
+            iter_l. rewrite list_lookup_insert /=; [|rewrite length_fmap //].
+            step_l. unshelve eexists; eauto. norm_l. step_l. norm_l.
+            rewrite list_insert_insert.
+
+            iter_l. rewrite list_lookup_insert /=; [|rewrite length_fmap //].
+            step_l. norm_l.
+            rewrite list_insert_insert. hss. ired. hss. ired.
+
+            iter_l. rewrite list_lookup_insert /=; [|rewrite length_fmap //].
+            step_l. norm_l.
+            rewrite list_insert_insert. ired.
+
+            iter_r. rewrite list_lookup_insert /=; [|rewrite length_fmap //]. step_r.
+            iter_l. rewrite list_lookup_insert /=; [|rewrite length_fmap //]. step_l.
+            rewrite {1 3}/LMod.prog /=.
+
+            destruct (dec _ _); [exfalso; hexploit yield_run_neq; ii; clarify|].
+            destruct (dec _ _); [exfalso; hexploit yield_help_neq; ii; clarify|ss].
+            norm_l. norm_r.
+            rewrite /ModTr.trans_ktree /SB.sandbox_body /ModTr.trans /SB.sandbox /=.
+            rewrite ?list_insert_insert. ired.
+
+            (* enter SchI yield - tgt *)
+            rewrite /SchI.yield /SchI.SchI.trigger_Yield.
+
+            iter_l. rewrite list_lookup_insert /=; [|rewrite length_fmap //].
+            step_l. norm_l.
+            rewrite ?list_insert_insert.
+
+            iter_r. rewrite list_lookup_insert /=; [|rewrite length_fmap //]. step_r. norm_r.
+            rewrite ?list_insert_insert.
+
+            rewrite /cfunU. destruct (arg ↓) eqn : Harg; cycle 1.
+            { iter_l. rewrite list_lookup_insert /=; [|rewrite length_fmap //].
+              destruct (sumbool_to_bool _); ss; step_l; ss.
+            }
+            ss. ired.
+
+            iter_r. rewrite list_lookup_insert /=; [|rewrite length_fmap //]. step_r. norm_r.
+            rewrite list_insert_insert. hss. rewrite ModTr.alist_encode_decode /=.
+            ired. hss. ired.
+
+            iter_r. rewrite list_lookup_insert /=; [|rewrite length_fmap //]. step_r.
+            intros [tid_nxt Htid_nxt]. norm_r. step_r. norm_r.
+            rewrite list_insert_insert. ired.
+
+            iter_r. rewrite list_lookup_insert /=; [|rewrite length_fmap //]. step_r. norm_r.
+            rewrite list_insert_insert. hss. rewrite ModTr.alist_encode_decode /=.
+            ired. hss. ired.
+
+            iter_r. rewrite list_lookup_insert /=; [|rewrite length_fmap //]. step_r. norm_r.
+            hss. rewrite ModTr.alist_encode_decode /=. ired. hss. ired.
+            destruct (nth_error _ _) as [stid_next|] eqn : Hnth; cycle 1.
+            { exfalso; eapply nth_error_Some in Htid_nxt; done. }
+            rewrite list_insert_insert.
+
+            iter_r. rewrite list_lookup_insert /=; [|rewrite length_fmap //].
+            step_r. norm_r. ired.
+            rewrite list_insert_insert.
+
+            iter_l. rewrite list_lookup_insert /=; [|rewrite length_fmap //].
+            step_l. norm_l. hss. rewrite ModTr.alist_encode_decode /=.
+            ired. hss. ired.
+            rewrite list_insert_insert.
+
+            iter_l. rewrite list_lookup_insert /=; [|rewrite length_fmap //].
+            step_l. exists (exist _ tid_nxt Htid_nxt). norm_l. step_l. norm_l.
+            rewrite list_insert_insert.
+
+            iter_l. rewrite list_lookup_insert /=; [|rewrite length_fmap //].
+            step_l. norm_l. hss. rewrite ModTr.alist_encode_decode.
+            rewrite list_insert_insert. ired. hss. ired.
+
+            iter_l. rewrite list_lookup_insert /=; [|rewrite length_fmap //].
+            step_l. norm_l. hss. rewrite ModTr.alist_encode_decode /=. ired. hss. ired.
+            rewrite list_insert_insert. rewrite Hnth /=. ired.
+
+            iter_l. rewrite list_lookup_insert /=; [|rewrite length_fmap //].
+            step_l. norm_l.
+            rewrite list_insert_insert. ired.
+
+            iter_l. rewrite list_lookup_insert /=; [|rewrite length_fmap //].
+            step_l. norm_l.
+            rewrite list_insert_insert. ired.
+
+            iter_r. rewrite list_lookup_insert /=; [|rewrite length_fmap //].
+            step_r. norm_r.
+            rewrite list_insert_insert. ired.
+
+            gbase. eapply (CIH rs_2); eauto.
+            set (tid_stid_cur := fresh _).
+            eset (tl2 := <[stid_cur := (_, _, Some (tid_stid_cur, j, None))]> tl).
+            assert (Htl2 : NoDup (to_reqlist tl2).*1).
+            { rewrite /tl2.
+              rewrite insert_take_drop // /to_reqlist fmap_app fmap_cons /=.
+              rewrite omap_app /=.
+              rewrite cons_app Permutation_app_swap_app /=; econs.
+              { subst tid_stid_cur; rewrite /to_reqmap /to_reqlist.
+                erewrite <-(take_drop_middle tl stid_cur) at 1; eauto.
+                rewrite fmap_app omap_app; simpl omap.
+                rewrite -omap_app -fmap_app.
+                apply not_elem_of_list_to_map, not_elem_of_dom, is_fresh.
+              }
+              { revert Htl.
+                erewrite <-(take_drop_middle tl stid_cur) at 1; eauto.
+                rewrite /to_reqlist.
+                rewrite fmap_app omap_app /= -NoDup_ListNoDup //.
+              }
+            }
+            eexists tl2; esplits; eauto.
+            { repeat f_equal.
+              subst tl2.
+              rewrite /to_reqmap /to_reqlist.
+              erewrite <-(take_drop_middle tl stid_cur) at 1; eauto.
+              rewrite insert_take_drop; last ss.
+              rewrite /to_reqmap /to_reqlist /= !fmap_app !omap_app /=.
+              fold (to_reqlist (take stid_cur tl)).
+              fold (fmap snd (drop (S stid_cur) tl)).
+              set (f := λ _, _). fold (omap f (drop (S stid_cur) tl).*2).
+              rewrite /HelpingOn.jobmap; symmetry; apply map_to_list_insert_inv.
+              rewrite map_to_list_to_map.
+              { rewrite cons_app Permutation_app_swap_app //=. }
+              revert Htl2.
+              rewrite insert_take_drop // {1}/to_reqlist fmap_app omap_app //=.
+            }
+            { rewrite list_fmap_insert //=. }
+            { rewrite list_fmap_insert //=. }
+            { rewrite -NoDup_ListNoDup //. }
+            { intros i; destruct (decide (i = stid_cur)); subst; cycle 1.
+              { intros ???; rewrite list_lookup_insert_ne //=; apply Hlookup. }
+              { rewrite list_lookup_insert; ii; clarify; r; esplits; eauto.
+                { rewrite /helpee_pend_s. grind. repeat f_equal.
+                  { rewrite /yield_epliogue; grind. extensionality a; grind. }
+                  { instantiate (1:=k). extensionality a; grind. }
+                }
+                { rewrite /helpee_pend_t. grind. repeat f_equal.
+                  { extensionality a; grind. }
+                  { extensionality a; grind. }
+                }
+              }
+            }
+          }
+          { (* no sp *)
+            ired.
+
+            iter_r. rewrite list_lookup_insert /=; [|rewrite length_fmap //]. step_r.
+            iter_l. rewrite list_lookup_insert /=; [|rewrite length_fmap //]. step_l.
+            rewrite {1 3}/LMod.prog /=.
+
+            destruct (dec _ _); [exfalso; hexploit yield_run_neq; ii; clarify|].
+            destruct (dec _ _); [exfalso; hexploit yield_help_neq; ii; clarify|ss].
+            norm_l. norm_r.
+            rewrite /ModTr.trans_ktree /SB.sandbox_body /ModTr.trans /SB.sandbox /=.
+            rewrite ?list_insert_insert. ired.
+
+            rewrite /SchI.SchI.yield /cfunN /cfunU. hss. ired.
+
+            iter_r. rewrite list_lookup_insert /=; [|rewrite length_fmap //].
+            step_r. norm_r.
+            rewrite list_insert_insert.
+
+            iter_r. rewrite list_lookup_insert /=; [|rewrite length_fmap //].
+            step_r. norm_r. hss. rewrite ModTr.alist_encode_decode.
+            rewrite list_insert_insert. ired. hss. ired.
+
+            iter_r. rewrite list_lookup_insert /=; [|rewrite length_fmap //]. step_r.
+            intros [tid_nxt Htid_nxt]. norm_r. step_r. norm_r.
+            rewrite list_insert_insert. ired.
+
+            iter_r. rewrite list_lookup_insert /=; [|rewrite length_fmap //]. step_r. norm_r.
+            rewrite list_insert_insert. hss. rewrite ModTr.alist_encode_decode /=.
+            ired. hss. ired.
+
+            iter_r. rewrite list_lookup_insert /=; [|rewrite length_fmap //]. step_r. norm_r.
+            hss. rewrite ModTr.alist_encode_decode /=. ired. hss. ired.
+            destruct (nth_error _ _) as [stid_next|] eqn : Hnth; cycle 1.
+            { exfalso; eapply nth_error_Some in Htid_nxt; done. }
+            rewrite list_insert_insert.
+
+            iter_r. rewrite list_lookup_insert /=; [|rewrite length_fmap //].
+            step_r. norm_r. ired.
+            rewrite list_insert_insert.
+            
+            iter_l. rewrite list_lookup_insert /=; [|rewrite length_fmap //].
+            step_l. norm_l.
+            rewrite list_insert_insert. ired.
+
+            iter_l. rewrite list_lookup_insert /=; [|rewrite length_fmap //].
+            step_l. norm_l. hss. rewrite ModTr.alist_encode_decode.
+            rewrite list_insert_insert. ired. hss. ired.
+
+            iter_l. rewrite list_lookup_insert /=; [|rewrite length_fmap //].
+            step_l. exists (exist _ tid_nxt Htid_nxt). norm_l. step_l. norm_l.
+            rewrite list_insert_insert.
+
+            iter_l. rewrite list_lookup_insert /=; [|rewrite length_fmap //].
+            step_l. norm_l. hss. rewrite ModTr.alist_encode_decode /=. ired. hss. ired.
+            rewrite list_insert_insert. rewrite /cgetU.
+
+            iter_l. rewrite list_lookup_insert /=; [|rewrite length_fmap //].
+            step_l. norm_l. rewrite list_insert_insert. ired. hss.
+            rewrite ModTr.alist_encode_decode /=. ired. hss. ired. rewrite Hnth. ired.
+
+            iter_l. rewrite list_lookup_insert /=; [|rewrite length_fmap //].
+            step_l. norm_l.
+            rewrite list_insert_insert. ired.
+
+            iter_l. rewrite list_lookup_insert /=; [|rewrite length_fmap //].
+            step_l. norm_l.
+            rewrite list_insert_insert. ired.
+
+            iter_r. rewrite list_lookup_insert /=; [|rewrite length_fmap //].
+            step_r. norm_r.
+            rewrite list_insert_insert. ired.
+
+            gbase. eapply (CIH rs); eauto.
+            set (tid_stid_cur := fresh _).
+            eset (tl2 := <[stid_cur := (_, _, Some (tid_stid_cur, j, None))]> tl).
+            assert (Htl2 : NoDup (to_reqlist tl2).*1).
+            { rewrite /tl2.
+              rewrite insert_take_drop // /to_reqlist fmap_app fmap_cons /=.
+              rewrite omap_app /=.
+              rewrite cons_app Permutation_app_swap_app /=; econs.
+              { subst tid_stid_cur; rewrite /to_reqmap /to_reqlist.
+                erewrite <-(take_drop_middle tl stid_cur) at 1; eauto.
+                rewrite fmap_app omap_app; simpl omap.
+                rewrite -omap_app -fmap_app.
+                apply not_elem_of_list_to_map, not_elem_of_dom, is_fresh.
+              }
+              { revert Htl.
+                erewrite <-(take_drop_middle tl stid_cur) at 1; eauto.
+                rewrite /to_reqlist.
+                rewrite fmap_app omap_app /= -NoDup_ListNoDup //.
+              }
+            }
+            eexists tl2; esplits; eauto.
+            { repeat f_equal.
+              subst tl2.
+              rewrite /to_reqmap /to_reqlist.
+              erewrite <-(take_drop_middle tl stid_cur) at 1; eauto.
+              rewrite insert_take_drop; last ss.
+              rewrite /to_reqmap /to_reqlist /= !fmap_app !omap_app /=.
+              fold (to_reqlist (take stid_cur tl)).
+              fold (fmap snd (drop (S stid_cur) tl)).
+              set (f := λ _, _). fold (omap f (drop (S stid_cur) tl).*2).
+              rewrite /HelpingOn.jobmap; symmetry; apply map_to_list_insert_inv.
+              rewrite map_to_list_to_map.
+              { rewrite cons_app Permutation_app_swap_app //=. }
+              revert Htl2.
+              rewrite insert_take_drop // {1}/to_reqlist fmap_app omap_app //=.
+            }
+            { rewrite list_fmap_insert //=. }
+            { rewrite list_fmap_insert //=. }
+            { rewrite -NoDup_ListNoDup //. }
+            { intros i; destruct (decide (i = stid_cur)); subst; cycle 1.
+              { intros ???; rewrite list_lookup_insert_ne //=; apply Hlookup. }
+              { rewrite list_lookup_insert; ii; clarify; r; esplits; eauto.
+                { rewrite /helpee_pend_s. grind. repeat f_equal.
+                  { extensionality a; grind. }
+                  { instantiate (1:=k). extensionality a; grind. }
+                }
+                { rewrite /helpee_pend_t. grind. repeat f_equal.
+                  { extensionality a; grind. }
+                  { extensionality a; grind. }
+                }
+              }
+            }
+          }
+        }
+
+        destruct (decide (fn = Helping.help mn)) as [->|Hfn].
+        { (* Helping *)
+          rewrite {1 3}/LMod.prog /=.
+          destruct (dec _ _); [exfalso; ii; clarify|].
+          destruct (dec _ _); ss.
+          norm_l; norm_r.
+          rewrite /ModTr.trans_ktree /ModTr.trans /SB.sandbox_body /SB.sandbox /=.
+          rewrite /HelpingOn.help /HelpingOff.help.
+
+          iter_l. rewrite list_lookup_insert /=; [|rewrite length_fmap //]. step_l. norm_l.
+          rewrite list_insert_insert.
+
+          iter_r. rewrite list_lookup_insert /=; [|rewrite length_fmap //]. step_r. norm_r.
+          rewrite list_insert_insert.
+
+          iter_r. rewrite list_lookup_insert /=; [|rewrite length_fmap //].
+          step_r. intros tid_helpee. norm_r. step_r. norm_r.
+          rewrite list_insert_insert. ired.
+
+          destruct ((to_reqmap tl) !! tid_helpee) as [[jid_helpee [|]] |] eqn : Hhelpee; ss.
+          { (* Found one to help *)
+            rewrite {1}yield_unfold.
+
+            iter_l. rewrite list_lookup_insert /=; [|rewrite length_fmap //]. step_l. norm_l.
+            rewrite list_insert_insert.
+
+            iter_l. rewrite list_lookup_insert /=; [|rewrite length_fmap //]. step_l.
+            exists (Some true). norm_l. step_l. norm_l.
+            rewrite list_insert_insert. ired.
+
+            iter_l. rewrite list_lookup_insert /=; [|rewrite length_fmap //]. step_l. norm_l.
+            rewrite list_insert_insert.
+
+            rewrite HoareCall_unfold. ired.
+            rewrite /HoareCall_prologue; unseal "Help"; destruct (sp SchHdr.yield) as [yield_spec|].
+            { 
+              iter_r. rewrite list_lookup_insert /=; [|rewrite length_fmap //].
+              step_r. intros x. norm_r. step_r. norm_r.
+              rewrite list_insert_insert.
+
+              iter_r. rewrite list_lookup_insert /=; [|rewrite length_fmap //].
+              step_r. intros arg. norm_r. step_r. norm_r.
+              rewrite list_insert_insert.
+
+              iter_r. rewrite list_lookup_insert /=; [|rewrite length_fmap //].
+              step_r. norm_r.
+              rewrite list_insert_insert. hss. ired. hss. ired.
+
+              iter_r. rewrite list_lookup_insert /=; [|rewrite length_fmap //].
+              step_r. intros rs_2. norm_r. step_r. norm_r.
+              rewrite list_insert_insert.
+
+              iter_r. rewrite list_lookup_insert /=; [|rewrite length_fmap //].
+              step_r. intros Hrs_2. norm_r. step_r. norm_r.
+              rewrite list_insert_insert.
+
+              iter_r. rewrite list_lookup_insert /=; [|rewrite length_fmap //].
+              step_r. norm_r.
+              rewrite list_insert_insert. hss. ired. hss. ired.
+
+              iter_r. rewrite list_lookup_insert /=; [|rewrite length_fmap //].
+              step_r. norm_r.
+              rewrite list_insert_insert. ired.
+
+              iter_l. rewrite list_lookup_insert /=; [|rewrite length_fmap //].
+              step_l. exists x. norm_l. step_l. norm_l.
+              rewrite list_insert_insert.
+
+              iter_l. rewrite list_lookup_insert /=; [|rewrite length_fmap //].
+              step_l. exists arg. norm_l. step_l. norm_l.
+              rewrite list_insert_insert.
+
+              iter_l. rewrite list_lookup_insert /=; [|rewrite length_fmap //].
+              step_l. norm_l.
+              rewrite list_insert_insert. hss. ired. hss. ired.
+
+              iter_l. rewrite list_lookup_insert /=; [|rewrite length_fmap //].
+              step_l. exists rs_2. norm_l. step_l. norm_l.
+              rewrite list_insert_insert.
+
+              iter_l. rewrite list_lookup_insert /=; [|rewrite length_fmap //].
+              step_l. unshelve eexists; eauto. norm_l. step_l. norm_l.
+              rewrite list_insert_insert.
+
+              iter_l. rewrite list_lookup_insert /=; [|rewrite length_fmap //].
+              step_l. norm_l.
+              rewrite list_insert_insert. hss. ired. hss. ired.
+
+              iter_l. rewrite list_lookup_insert /=; [|rewrite length_fmap //].
+              step_l. norm_l.
+              rewrite list_insert_insert. ired.
+
+              iter_l. rewrite list_lookup_insert /=; [|rewrite length_fmap //].
+              step_l. norm_l.
+              rewrite {1}/LMod.prog /=.
+              destruct (dec _ _); [exfalso; hexploit yield_run_neq; ii; clarify|].
+              destruct (dec _ _); [exfalso; hexploit yield_help_neq; ii; clarify|ss].
+              norm_l.
+              rewrite list_insert_insert.
+              rewrite /ModTr.trans_ktree /SB.sandbox_body /ModTr.trans /SB.sandbox /=.
+
+              iter_l. rewrite list_lookup_insert /=; [|rewrite length_fmap //].
+              step_l. norm_l.
+              rewrite list_insert_insert. ired.
+
+              (* Source yield only *)
+              rewrite /SchI.yield /cfunU /SchI.SchI.trigger_Yield.
+              destruct (arg ↓); cycle 1.
+              { ss. iter_l. rewrite list_lookup_insert /=; [|rewrite length_fmap //].
+                destruct (sumbool_to_bool _); ss; step_l; ss.
+              }
+              ss. norm_l. ired.
+
+              iter_l. rewrite list_lookup_insert /=; [|rewrite length_fmap //].
+              step_l. norm_l. rewrite list_insert_insert. ired. hss.
+              rewrite ModTr.alist_encode_decode /=. ired. hss. ired.
+            }
+            admit.
+          }
+        admit.
+      }
+
+      { (* Spawn case *)
+        ss.
+        admit.
+      }
+
+      { (* Yield case *)
+        admit.
+      }
+
+      destruct Hf as [[R [s [f' ->]]]|[R [e [f' ->]]]].
+      { (* sput sget *)
+        admit.
+      }
+
+      destruct e; admit.
     }
-    destruct Hf as [[f' ->]|Hf].
-    { zprogress. ziter_l. zstep_l.
-      ziter_r; zstep_r. gbase.
-      rewrite /ModTr.trans. eapply CIH; eauto.
+
+    destruct p as [[tid jid] [[|]|]].
+    { (* Helpee *)
+      apply lookup_lt_Some in Htid as Htid_cur.
+      pose proof Htid as Htid'.
+      apply Hlookup in Htid' as [-> ->]; ss.
+      admit.
     }
+    { (* Helper *)
+      admit.
+    }
+    { (* Looping Helpee *)
+      admit.
+    }
+    Unshelve. exact smj_top.
+  Admitted.
+
+
+
     destruct Hf as [[P [f' ->]]|Hf].
     {
-      destruct imgf; [|ziter_l; zstep_l].
+      (* destruct imgf; [|ziter_l; zstep_l]. *)
       zprogress.
 
       iter_l. step_l. norm_l.
@@ -479,9 +1359,11 @@ Tactic Notation "red_ModTr" tactic(tac) :=
       iter_r. hss. norm_r. step_r. norm_r. ired.
 
       gbase. eapply (CIH res); des; eauto.
+      esplits; eauto.
     }
     destruct Hf as [[res [f' ->]]|Hf].
-    { rewrite !SBRed.bind ?SBRed.AssumeRes.
+    { 
+      (* rewrite !SBRed.bind ?SBRed.AssumeRes. *)
       zprogress.
       iter_l. step_l. norm_l.
       iter_l. hss. hss. norm_l. step_l. intros Hval. norm_l. step_l. norm_l.
@@ -493,9 +1375,11 @@ Tactic Notation "red_ModTr" tactic(tac) :=
       iter_r. step_r. norm_r.
       iter_r. hss. norm_r. step_r. norm_r.
       ired. gbase. eapply (CIH (res ⋅ rs)); des; eauto.
+      esplits; eauto.
     }
     destruct Hf as [[P [f' ->]]|Hf].
-    { rewrite !SBRed.bind !SBRed.Guarantee.
+    {
+      (* rewrite !SBRed.bind !SBRed.Guarantee. *)
       zprogress.
       iter_r. step_r. norm_r.
       iter_r. hss. hss. step_r. intros x. norm_r. step_r. norm_r.
@@ -510,39 +1394,244 @@ Tactic Notation "red_ModTr" tactic(tac) :=
       iter_l. hss. step_l. norm_l.
       ired.
       gbase. eapply (CIH x); des; eauto.
+      esplits; eauto.
     }
     destruct Hf as [[R [[fn args|fn args|tid_yield] [k ->]]]|Hf].
-    { rewrite !SBRed.bind !SBRed.call.
-      destruct (mskf fn) eqn : Hmask; [|iter_l; step_l; ss].
+    { 
+      (* rewrite !SBRed.bind !SBRed.call. *)
+      (* destruct (mskf fn) eqn : Hmask; [|iter_l; step_l; ss]. *)
+      zprogress.
 
       iter_l. step_l. iter_r. step_r.
       rewrite /HelpingOff.t /SchA.t /HelpingOn.t /=; unseal CRIS; ss.
       destruct (decide (fn = Helping.run mn)); subst.
-      {
-        norm_l. norm_r.
+      { norm_l. norm_r.
         rewrite {1 3}/LMod.prog ?alist_find_map_snd /=.
         destruct (dec _ _) as [?|e]; [ss|clarify].
         norm_l. norm_r.
 
+        replace_tp_r.
+        { instantiate (1:=(0, [x <- _;; after_call k x])).
+          repeat f_equal. rewrite /after_call; extensionalities i; repeat f_equal; grind.
+        }
+        replace_tp_l.
+        { instantiate (1:=(0, [x <- _;; after_call k x])).
+          repeat f_equal. rewrite /after_call; extensionalities i; repeat f_equal; grind.
+        }
+
         iter_r. step_r. norm_r.
         rewrite /HelpingOn.run /HelpingOff.run.
         destruct (args↓) as [j|] eqn:Hargs ; cycle 1.
-        { iter_l. step_l. norm_l. iter_l. rewrite Hargs /=. des_if; norm_l; step_l; ss. }
+        { iter_l. step_l. norm_l. iter_l. rewrite Hargs /=. norm_l; step_l; ss. }
         ss.
+        rewrite /ModTr.trans_ktree /SB.sandbox_body /= Hargs.
 
+        iter_l. step_l. norm_l. ired.
+        (* rewrite {1 2}yield_unfold. *)
+        (* rewrite /Sch.yield; unseal "Sch". *)
+
+        iter_r. rewrite String.eqb_refl /=. step_r. norm_r. hss. rewrite ModTr.alist_encode_decode.
+        ss. destruct (dec _ _) as [e|]; ss; clear e.
+        iter_r. hss. rewrite String.eqb_refl /=. norm_r. step_r. norm_r. hss.
         iter_r. step_r. norm_r.
         iter_r. step_r. norm_r.
 
-        rewrite {2}/LMod.prog ?alist_find_map_snd /=.
+        set (loop := λ _ : (), _) at 4.
+        rewrite (bisim_is_eq (unfold_iter _ _)).
+        ired.
+        (* rewrite {12}unfold_iterC. *)
+        (* iter_r. step_r. norm_r. ired.
+        iter_l. step_l. norm_l. *)
 
+        gcofix CIH2.
 
-        rewrite /Sch.yield; unseal "Sch".
-        rewrite unfold_iterC.
-        norm_l. step_l.
-        norm_l. iter_l.
+        rewrite {2}yield_unfold.
+        iter_r. step_r. norm_r.
+        iter_r. step_r. intros [b|]; cycle 1.
+        { clear CIH2.
+          step_r. norm_r. iter_r.
+          rewrite String.eqb_refl /=. step_r. norm_r. hss.
+          rewrite ?ModTr.alist_encode_decode.
+          erewrite (alist_upd_find); cycle 1.
+          { ss; destruct (dec _ _); ss. }
+          ss. grind. hss. grind.
+          rewrite lookup_insert /=.
+          iter_r. rewrite String.eqb_refl /=. step_r. norm_r.
+          hss. rewrite ModTr.alist_encode_decode /=.
+          erewrite (alist_upd_find); cycle 1.
+          { ss; destruct (dec _ _); ss. }
+          ss. grind. hss. grind.
+          rewrite delete_insert.
+          2:{ rewrite -not_elem_of_dom; eapply is_fresh. }
+          rewrite lookup_insert //=.
+          iter_r. rewrite String.eqb_refl /=. step_r. norm_r.
+          hss. iter_r. step_r. norm_r. grind. rewrite ModTr.alist_encode_decode.
+          rewrite alist_shadow alist_find_upd //=; cycle 1.
+          { destruct (dec _ _); ss. }
+
+          rewrite yield_unfold.
+          iter_l. step_l. norm_l.
+          iter_l. step_l. exists None. step_l. norm_l.
+          ired.
+          gbase.
+          set (f1 := (0, _)). pattern f1. eapply eq_ind_r.
+          { eapply (CIH rs Hrs); esplits; eauto. }
+          { subst f1; f_equal; f_equal.
+            rewrite /ModTr.trans.
+            instantiate (1:= ITree.bind _ (λ x, tau;; _ x)).
+            rewrite (@interpV_bind _ _ _ Any.t ModTr.handle_crisE); f_equal.
+            extensionality x.
+            rewrite interpV_tau; do 2 f_equal.
+            (* rewrite ?bind_ret_l //. *)
+          }
+        }
+        destruct b; cycle 1.
+        { zprogress. norm_r. step_r. norm_r. ired.
+          rewrite {1}yield_unfold.
+          (* iter_r. step_r. norm_r. *)
+
+          iter_l. step_l. norm_l.
+          iter_l. step_l. exists (Some false). step_l. norm_l. ired.
+          gbase.
+          revert CIH2. rewrite /iterC.
+          set (f1 := (0, _)) at 2. set (f3 := (0, _)) at 3. assert (f1 = f3).
+          { subst f1 f3. f_equal. }
+          rewrite H0. clear f1 H0.
+          eauto.
+        }
+
+        clear CIH2.
+        step_r. norm_r.
+        iter_r. step_r. norm_r.
+
+        rewrite {1}yield_unfold.
+        iter_l. step_l. norm_l.
+        iter_l. norm_l. step_l. exists (Some true). norm_l. step_l. norm_l.
+        iter_l. step_l. norm_l.
+        rewrite ModTr.alist_encode_decode /alist_upd /_alist_upd; ss; destruct (dec _ _); ss.
+
+        rewrite HoareCall_unfold. ired.
+        rewrite /HoareCall_prologue; unseal "Help".
+
+        destruct (sp SchHdr.yield) as [yield_spec|].
+        { iter_r. step_r. intros x. norm_r. step_r. norm_r.
+          iter_r. step_r. intros arg. norm_r. step_r. norm_r.
+          iter_r. step_r. norm_r. hss.
+          iter_r. hss. step_r. intros rs_2. norm_r. step_r. norm_r.
+          iter_r. step_r. intros Hrs_2. norm_r. step_r. norm_r.
+          iter_r. step_r. norm_r. iter_r. hss. step_r. norm_r. ired.
+
+          iter_l. step_l. exists x. norm_l. step_l. norm_l.
+          iter_l. step_l. exists arg. norm_l. step_l. norm_l.
+          iter_l. step_l. norm_l. hss.
+          iter_l. hss. step_l. exists rs_2. norm_l. step_l. norm_l.
+          iter_l. step_l. unshelve eexists; eauto. norm_l. step_l. norm_l.
+          iter_l. step_l. norm_l. iter_l. hss. step_l. norm_l. ired.
+
+          iter_r. step_r. iter_l. step_l.
+          rewrite {1 3}/LMod.prog /=.
+
+          destruct (dec _ _); [exfalso; hexploit yield_run_neq; ii; clarify|].
+          destruct (dec _ _); [exfalso; hexploit yield_help_neq; ii; clarify|ss].
+          norm_l. norm_r.
+          iter_l. step_l. intros tid. norm_l. step_l. norm_l.
+          iter_l. step_l. intros arg_y. norm_l. step_l. norm_l.
+          iter_l. step_l. norm_l. hss.
+          iter_l. hss. norm_l. step_l. intros rs_3. norm_l. step_l. norm_l.
+          iter_l. step_l. intros Hrs_3. norm_l. step_l. norm_l.
+
+          iter_r. step_r. exists tid. norm_r. step_r. norm_r.
+          iter_r. step_r. exists arg_y. norm_r. step_r. norm_r.
+          iter_r. step_r. norm_r. hss.
+          iter_r. hss. step_r. exists rs_3. norm_r. step_r. norm_r.
+          iter_r. step_r. unshelve eexists; eauto. norm_r. step_r. norm_r.
+          iter_r. step_r. norm_r. iter_r. hss. step_r. norm_r. ired.
+          rewrite /SchI.SchI.yield.
+          iter_r. destruct (arg_y ↓) eqn : Harg_y; cycle 1.
+          { ss. step_r; ss. }
+          ss. step_r. norm_r. hss. rewrite ModTr.alist_encode_decode /=.
+          ired. hss. iter_r. step_r. intros [tid_next Htid_next]. norm_r. step_r. norm_r.
+          iter_r. step_r. norm_r. hss. rewrite ModTr.alist_encode_decode /=.
+          rewrite /alist_upd /_alist_upd /=. iter_r. step_r. norm_r.
+          rewrite /SchI.SchI.trigger_Yield.
+          iter_r. step_r. norm_r. hss. rewrite ModTr.alist_encode_decode /=. ired. hss.
+          iter_r. step_r. norm_r. hss. rewrite ModTr.alist_encode_decode /=. ired. hss.
+          ired. destruct (nth_error _ _) as [stid_next|] eqn : Hnth; cycle 1.
+          { exfalso; eapply nth_error_Some in Htid_next; done. }
+          iter_r. step_r. norm_r. ired.
+
+          iter_l. step_l. norm_l.
+          ired. hss. ired. iter_l. step_l. norm_l.
+          rewrite /cfunN. hss. iter_l. step_l. norm_l. hss. rewrite ModTr.alist_encode_decode /=.
+          ired. hss. ired.
+          iter_l. step_l.
+          exists (exist _ tid_next Htid_next). norm_l. step_l. norm_l.
+          rewrite /SchA.trigger_Yield /SchI.SchI.trigger_Yield.
+          iter_l. step_l. norm_l. hss. rewrite ModTr.alist_encode_decode.
+          iter_l. step_l. norm_l.
+          iter_l. step_l. norm_l. hss. rewrite ModTr.alist_encode_decode.
+          rewrite /alist_upd /_alist_upd /=. ired. hss.
+          iter_l. step_l. norm_l. hss. rewrite ModTr.alist_encode_decode /=. ired. hss.
+          ired. rewrite Hnth. ired.
+          iter_l. step_l. norm_l.
+          iter_l. step_l. norm_l.
+          iter_r. step_r. norm_r.
+          ired.
+
+          Definition yield_epliogue (tid_cur tid : nat) : itree crisE Any.t :=
+            cput SchI.SchI.v_tid tid_cur;;;
+            x <- SchA.check_internal;;
+            ret <- trigger (Choose Any.t);;
+            trigger (Guarantee (postcond (SchAS.yield_spec ⊤ 1) tid (()↑) ret));;;
+            Ret ret.
+
+          replace_tp_r.
+          { instantiate (1:=
+              (_,
+              [ret <- interpV ModTr.handle_crisE
+                (interpV (SB.handle_sandbox true _ SchA.scopes)
+                  (interpV (SModTr.handle sp_s) (yield_epliogue tid_cur tid)));;
+               ret <-interpV ModTr.handle_crisE
+                (interpV (SB.handle_sandbox true wmask_all (HelpingOn.scopes mn))
+                  (interpV (SModTr.handle sp)
+                    (tau;; HoareCall_epilogue (Some yield_spec) x ret;;;
+                     𝒴;;;
+                     cond <- loop ();;
+                     match cond with
+                     | inl l => tau;; ITree.iter (λ _ : (), x <- 𝒴;; loop x) l
+                     | inr r1 => Ret r1
+                     end;;;
+                     HelpingOn.try_run mn jobs (fresh (dom tidmap))
+                    )));;
+                after_call k ret
+              ])). do 2 f_equal. f_equal.
+            { do 2 f_equal.
+              rewrite /yield_epliogue; ired.
+              rewrite ?interpV_bind; ired. grind.
+              rewrite interpV_ret; ired.
+              rewrite interpV_trigger /=; ired; grind.
+              rewrite interpV_bind interpV_trigger /=. ired. destruct x0, x3. f_equal.
+              rewrite interpV_ret; extensionalities a; destruct a; ired. done.
+            }
+            { extensionalities ret. ired.
+              rewrite ?interpV_tau. do 2 f_equal.
+              rewrite interpV_bind; ired. rewrite interpV_bind. ired.
+              rewrite (interpV_bind (SModTr.handle sp) (HoareCall_epilogue _ _ _)).
+              etransitivity; last (rewrite interpV_bind; refl).
+              etransitivity; last (rewrite interpV_bind; refl). do 2 f_equal.
+              rewrite bind_bind. f_equal.
+
+              { do 2 f_equal. rewrite /HoareCall_epilogue; unseal "Help".
+                rewrite ?interpV_bind ?interpV_vis; ired; grind.
+                rewrite interpV_ret; ired.
+                rewrite interpV_bind interpV_vis interpV_ret; grind.
+                rewrite interpV_ret; grind.
+              }
+              extensionalities a. grind.
+            }
+          }
+        }
       }
     }
-
-
   Admitted.
 End Helping.
